src/riot/x509/X509.ExtFields.AuthorityKeyIdentifier.fsti
@@ -1,0 +1,160 @@
+module X509.ExtFields.AuthorityKeyIdentifier
+
+open ASN1.Spec
+open ASN1.Low
+
+open X509.Base
+
+open FStar.Integers
+
+//open X509.BasicFields.RelativeDistinguishedName
+//open X509.BasicFields.SerialNumber
+
+(* 4.2.1.1.  Authority Key Identifier
+
+   ...
+
+   The value of the keyIdentifier field SHOULD be derived from the
+   public key used to verify the certificate's signature or a method
+   that generates unique values.  Two common methods for generating key
+   identifiers from the public key are described in Section 4.2.1.2.
+   Where a key identifier has not been previously established, this
+   specification RECOMMENDS use of one of these methods for generating
+   keyIdentifiers or use of a similar method that uses a different hash
+   algorithm.  Where a key identifier has been previously established,
+   the CA SHOULD use the previously established identifier.
+
+   This profile RECOMMENDS support for the key identifier method by all
+   certificate users.
+
+   Conforming CAs MUST mark this extension as non-critical.
+
+   id-ce-authorityKeyIdentifier OBJECT IDENTIFIER ::=  { id-ce 35 }
+
+   AuthorityKeyIdentifier ::= SEQUENCE {
+      keyIdentifier             [0] KeyIdentifier           OPTIONAL,
+      authorityCertIssuer       [1] GeneralNames            OPTIONAL,
+      authorityCertSerialNumber [2] CertificateSerialNumber OPTIONAL  }
+
+   KeyIdentifier ::= OCTET STRING
+
+ *)
+
+let x509_authKeyID_keyIdentifier_tag: asn1_tag_t
+= (CUSTOM_TAG CONTEXT_SPECIFIC CONSTRUCTED 0uy)
+
+(* Not supporting them for now *)
+// let x509_authKeyID_CertIssuer_tag: asn1_tag_t
+// = (CUSTOM_TAG CONTEXT_SPECIFIC CONSTRUCTED 1uy)
+
+// let x509_authKeyID_CertSN_tag: asn1_tag_t
+// = (CUSTOM_TAG CONTEXT_SPECIFIC CONSTRUCTED 2uy)
+
+(* keyIdentifier *)
+
+let x509_authKeyID_keyIdentifier_t
+= x509_authKeyID_keyIdentifier_tag `inbound_envelop_tag_with_value_of`
+  (**) (serialize_asn1_TLV_of_type OCTET_STRING)
+
+noextract
+val parse_x509_authKeyID_keyIdentifier
+: parser (parse_asn1_envelop_tag_with_TLV_kind x509_authKeyID_keyIdentifier_tag) x509_authKeyID_keyIdentifier_t
+
+noextract
+val serialize_x509_authKeyID_keyIdentifier
+: serializer parse_x509_authKeyID_keyIdentifier
+
+val serialize32_x509_authKeyID_keyIdentifier_backwards
+: serializer32_backwards serialize_x509_authKeyID_keyIdentifier
+
+val lemma_serialize_x509_authKeyID_keyIdentifier_unfold
+  (x: x509_authKeyID_keyIdentifier_t)
+: Lemma (
+  predicate_serialize_asn1_envelop_tag_with_TLV_unfold
+    (x509_authKeyID_keyIdentifier_tag)
+    (serialize_asn1_TLV_of_type OCTET_STRING)
+    (x)
+)
+
+val lemma_serialize_x509_authKeyID_keyIdentifier_size
+  (x: x509_authKeyID_keyIdentifier_t)
+: Lemma (
+  predicate_serialize_asn1_envelop_tag_with_TLV_size
+    (x509_authKeyID_keyIdentifier_tag)
+    (serialize_asn1_TLV_of_type OCTET_STRING)
+    (x)
+)
+
+let valid_authKeyID_keyIdentifier_ingredients
+  (keyID: datatype_of_asn1_type OCTET_STRING)
+: Type0
+= length_of_asn1_primitive_TLV keyID
+  <= asn1_value_length_max_of_type x509_authKeyID_keyIdentifier_tag
+
+let len_of_x509_authKeyID_keyIdentifier
+  (keyID: datatype_of_asn1_type OCTET_STRING
+          { valid_authKeyID_keyIdentifier_ingredients keyID })
+: Tot (asn1_TLV_int32_of_type x509_authKeyID_keyIdentifier_tag)
+= len_of_TLV
+    (x509_authKeyID_keyIdentifier_tag)
+    (len_of_asn1_primitive_TLV keyID)
+
+val lemma_serialize_x509_authKeyID_keyIdentifier_size_exact
+  (x: x509_authKeyID_keyIdentifier_t)
+: Lemma (
+  length_of_opaque_serialization serialize_x509_authKeyID_keyIdentifier x ==
+  (v (len_of_x509_authKeyID_keyIdentifier x))
+)
+
+let x509_get_authKeyID_keyIdentifier
+  (keyID: datatype_of_asn1_type OCTET_STRING
+          { valid_authKeyID_keyIdentifier_ingredients keyID })
+: Tot (x509_authKeyID_keyIdentifier_t)
+= keyID
+
+// let has_x509_keyIdentifier_t b
+// = if b then Some x509_keyIdentifier_t else None
+
+// let x509_generalNames_t
+// = (CUSTOM_TAG CONTEXT_SPECIFIC CONSTRUCTED 0uy) `inbound_envelop_tag_with_value_of`
+//   (**) (serialize_)
+
+// let x509_authorityCertSerialNumber_t
+// = (CUSTOM_TAG CONTEXT_SPECIFIC CONSTRUCTED 2uy) `inbound_envelop_tag_with_value_of`
+//   (**) (serialize_x509_serialNumber)
+
+
+// noextract inline_for_extraction
+// let x509_authKeyID_t
+//   (has_keyID: bool)
+//   (has_authCertSN: bool)
+// // : Type
+// = (has_x509_keyIdentifier_t
+//    `combine`
+//    has_x509_keyIdentifier_t)
+//   (has_keyID, has_authCertSN)
+
+
+// (* Example `DEFAULT` *)
+// let pd =
+//   parse_asn1_TLV_of_type INTEGER
+//   `parse_synth`
+//   (fun x -> match x with 0l -> None | _ -> Some x)
+
+// (* Example `OPTIONAL` *)
+// (* NOTE: This might be CSG, you need to look at explicit tag *)
+// (* NOTE: Statically determine this. *)
+
+// #push-options "--fuel 0 --ifuel 0"
+// let combine
+//   (#t1: Type)
+//   (f: t1 -> option Type)
+//   (#t2: Type)
+//   (g: t2 -> option Type)
+// : (t1 `tuple2` t2) -> option Type
+// = fun (a, b) ->
+//   match f a, g b with
+//   | Some x, Some y -> Some (x `tuple2` y)
+//   | Some x, None   -> Some x
+//   | None  , Some y -> Some y
+//   | None  , None   -> None
